\documentclass{article}
\usepackage{graphicx} % Required for inserting images
\usepackage{amsmath,amssymb,amsthm}
\usepackage{physics}
\usepackage{graphicx,float}
\graphicspath{{images/}}
\usepackage[none]{hyphenat}
\usepackage{blindtext}
\usepackage{parskip}
\usepackage[letterpaper,top=3cm, left= 3cm,bottom=3cm]{geometry}
\usepackage{subcaption}
\numberwithin{equation}{section}

\title{Partial Fraction}
\author{assassin3552}
\date{2025/03/29}

\begin{document}
\maketitle

Consider this integral:
\[
\int \frac{x + 1}{x^2 -5x + 6} \mathrm{d}x
\]
This integral looks scary, but notice that we can factor the denominator:
$x^2 - 5x + 6 = (x-2)(x-3)$

Let's first take at look at fraction addition:
\[
\frac{A}{B} + \frac{C}{D} = \frac{AD + BC}{BD}
\]
Since the integrand is a fraction, and we successfully write the denominator as a product,
we should be able to split the fraction into a sum of two fraction.

Assume we have split the fraction like this:
\[
\frac{x + 1}{(x - 2)(x - 3)} = \frac{A}{(x - 2)} + \frac{B}{(x - 3)}
\]
Here and $A$ and $B$ are different constant, let's try to combine them together:
\[
\frac{A(x - 3) +B(x - 2)}{(x - 2)(x - 3)} = \frac{Ax - 3A + Bx - 2B}{(x-2)(x-3)} = \frac{(A+B)x + (-3A-2B)}{(x-2)(x-3)}
\]

Notice that we reformed the denominator into $\text{constant} \cdot x + \text{constant}$, which does indeed look like $x+1$ in the original integrand,
thus we have this relation:
\[
\begin{cases}
    A+B = 1\\
    -3A - 2B = 1
\end{cases}
\]
This linear set of equation can be easily solved, which gives the solution of $A = -3$ and $B = 4$. Thus we turned this integrand into a fraction of sum:
\[
\int \frac{x + 1}{x^2 - 5x + 6} \mathrm{d}x= \int \left(-\frac{3}{(x - 2)} + \frac{4}{(x - 3)} \right) \mathrm{d}x
\]

Then we can evaluate the integral easily:
\[
\int \left(-\frac{3}{(x - 2)} + \frac{4}{(x - 3)} \right) \mathrm{d}x = -3\ln\abs{x-2} + 4\ln\abs{x-3} + C
\]

\newpage
In general, partial fraction follow this process:

Consider a integrand where the denominator can be factored, first split the fraction into a sum of fractions:
\[
\frac{Ax + B}{(x + C)(x + D)} = \frac{E}{(x + C)} + \frac{F}{(x + D)} = \frac{(E + F)x + (DE + CF)}{(x + C)(x + D)}
\]
Where $A, B, C, D, E, F$ are all constants, thus:
\[
\begin{cases}
    E + F = A\\
    DE + CF = B\\
\end{cases}
\]
Then solve for $E$ and $F$ to complete the fraction split.

Here is another example:
\[
\int \frac{2x - 1}{x^2 - 4x + 3} \mathrm{d}x = \int \frac{x + 1}{(x - 3)(x - 1)} \mathrm{d}x
\]
%so this is how to insert comment
Split the fraction into a sum of fraction:
\[
\frac{A}{x - 3} + \frac{B}{x - 1} = \frac{A(x - 1) + B(x - 3)}{(x - 3)(x - 1)} = \frac{(A+B)x +(-A -3B)}{(x-3)(x-1)}
\]
Solve for $A$ and $B$:
\[
\begin{cases}
    A+B = 1\\
    -A-3B = 1\\
\end{cases}
\]
Thus $A = 2$ and $B = -1$, and the integral turns to 
\[
\int \left(\frac{2}{x-3} - \frac{1}{x-1} \right) \mathrm{d}x = 2\ln\abs{x-3} - \ln\abs{x-1} + C
\]
\end{document}